behavior-preservation/FirstRisingEdge.v
@@ -15,7 +15,7 @@ Lemma first_rising_edge_full :
   forall sitpn id__ent id__arch b d γ E__c E__p Δ σ__e σ0 τ σ__i σ__r σ,
 
     (* sitpn translates into (d, γ). *)
-    sitpn_to_hvhdl sitpn id__ent id__arch b = (inl (d, γ)) ->
+    sitpn2hvhdl sitpn id__ent id__arch b = (inl (d, γ)) ->
 
     (* Environments are similar. *)
     SimEnv sitpn γ E__c E__p ->
@@ -44,7 +44,7 @@ Lemma first_rising_edge :
   forall sitpn id__ent id__arch b d γ E__c E__p Δ σ__e σ0 τ σ__i σ__r σ,
 
     (* sitpn translates into (d, γ). *)
-    sitpn_to_hvhdl sitpn id__ent id__arch b = (inl (d, γ)) ->
+    sitpn2hvhdl sitpn id__ent id__arch b = (inl (d, γ)) ->
 
     (* Environments are similar. *)
     SimEnv sitpn γ E__c E__p ->
