behavior-preservation/TraceSimilarity.v
@@ -49,7 +49,7 @@ Lemma trace_sim :
   forall sitpn id__ent id__arch b d γ E__c E__p Δ σ__e τ s σ θ__s θ__σ, 
 
     (* sitpn translates into (d, γ). *)
-    sitpn_to_hvhdl sitpn id__ent id__arch b = (inl (d, γ)) ->
+    sitpn2hvhdl sitpn id__ent id__arch b = (inl (d, γ)) ->
 
     (* Environments are similar. *)
     SimEnv sitpn γ E__c E__p ->
@@ -94,13 +94,13 @@ Qed.
     a given H-VHDL design [d]. *)
 
 Theorem full_trace_sim :
-  forall sitpn id__ent id__arch E__c τ θ__s d E__p b θ__σ γ Δ,
+  forall sitpn id__ent id__arch E__c τ θ__s d E__p b θ__σ γ,
 
     (* [sitpn] is well-defined. *)
     IsWellDefined sitpn ->
     
     (* sitpn translates into (d, γ). *)
-    sitpn_to_hvhdl sitpn id__ent id__arch b = (inl (d, γ)) ->
+    sitpn2hvhdl sitpn id__ent id__arch b = (inl (d, γ)) ->
 
     (* Environments are similar. *)
     SimEnv sitpn γ E__c E__p ->
@@ -110,35 +110,108 @@ Theorem full_trace_sim :
     @SitpnFullExec sitpn E__c τ θ__s ->    
     
     (* Design [d] yields simulation trace [θ__σ] after [τ] simulation cycles. *)
-    hfullsim E__p τ Δ d θ__σ ->
+    hfullsim E__p τ d θ__σ ->
     
     (* ** Conclusion: traces are positionally similar. ** *)
     FullSimTrace γ θ__s θ__σ.
 Proof.  
   (* Case analysis on τ *)
-  destruct τ;
-    intros *;
-    inversion_clear 4;
-    inversion_clear 1.
-
-  (* CASE τ = 0, GOAL [γ ⊢ s0 ∼ σ0]. Solved with [sim_init_states] lemma. *)
-  - lazymatch goal with
+  destruct τ; intros;
+  match goal with
+  | [ Hsitpn: SitpnFullExec _ _ _, Hd: hfullsim _ _ _ _
+      |- _ ] =>
+    inversion_clear Hsitpn; inversion_clear Hd
+  end;
+    lazymatch goal with
     | [ Hsimloop: simloop _ _ _ _ _ _ _ |- _ ] =>
-        inversion_clear Hsimloop;
-        constructor; eauto with hilecop
+        inversion_clear Hsimloop
     end.
+  (* CASE τ = 0, GOAL [γ ⊢ s0 ∼ σ0]. Solved with [sim_init_states] lemma. *)
+  - constructor; eauto with hilecop.
 
   (* CASE τ > 0, GOAL [γ ⊢ (s0 :: s :: θ__s) ∼ (σ0 :: σ :: θ0)].   
      Solved with [first_rising_edge], [falling_edge] and [trace_sim] lemmas. *)
     
-  - lazymatch goal with
+  - match goal with
+    | [ H: simcycle _ _ _ _ _ _ _ _ |- _ ] =>
+        inversion_clear H; repeat (constructor; eauto with hilecop)
+    end.
+
+Restart.
+
+  (* Version of the proof closer to the paper proof.
+
+     Induction on τ on the second part (no more appealing to lemma
+     [trace_sim]), and trying not to use the hilecop hint database. *)
+  destruct τ; intros;
+  match goal with
+  | [ Hsitpn: SitpnFullExec _ _ _, Hd: hfullsim _ _ _ _
+      |- _ ] =>
+    inversion_clear Hsitpn; inversion_clear Hd
+  end;
+    lazymatch goal with
     | [ Hsimloop: simloop _ _ _ _ _ _ _ |- _ ] =>
         inversion_clear Hsimloop
     end.
-    match goal with
+
+  (* CASE τ = 0, GOAL [ γ ⊢ [s0] ∼ [σ0] ] ⇒ [γ ⊢ s0 ≈ σ0]. 
+     Solved with [sim_init_states] lemma. *)
+  - eapply FullSimTraceCons; eauto.
+    eapply sim_init_states; eauto.
+
+  (* CASE τ > 0, GOAL [γ ⊢ (s0 :: s :: θ__s) ∼ (σ0 :: σ :: θ0)].   
+     Solved with [first_rising_edge], [falling_edge] and [trace_sim] lemmas. *)
+  - match goal with
     | [ H: simcycle _ _ _ _ _ _ _ _ |- _ ] =>
-        inversion_clear H; constructor; eauto with hilecop
+        inversion_clear H
     end.
-    constructor; eauto with hilecop.
-    constructor; eauto with hilecop.
+    (* SUBGOAL [γ ⊢ s0 ≈ σ0], solved with [sim_init_states]. *)
+    constructor. eapply sim_init_states; eauto.
+    (* SUBGOAL [γ ⊢ s0 ≈ σ'], solved with [first_rising_edge]. *)
+    constructor. eapply first_rising_edge; eauto.
+    (* SUBGOAL [γ ⊢ s ≈ σ''], solved with [falling_edge]. *)
+    constructor. eapply falling_edge; eauto with hilecop.
+    (* SUBGOAL [γ ⊢ θ ∼ θ1], induction on τ *)
+
+    (* Prepares the context and the goal to obtain the wanted
+       induction hypothesis. *)
+    assert (Hsimfe : FullSimStateAfterFE sitpn γ s σ'') by
+      (eauto with hilecop).
+
+    match goal with
+    | [
+        H0: SitpnStateTransition _ (S τ) _ _ _,
+          H1: IsInjectedDState _ (_ (S τ)) _,
+            H2: SitpnExecute _ ?s τ ?θ__s,
+              H3: simloop _ _ _ ?σ _ τ ?θ__σ,
+        H4: FullSimStateAfterFE _ _ ?s ?σ |- _
+      ] =>
+        clear H0 H1;
+        generalize H2 H3 H4; clear H2 H3 H4;
+        generalize s θ__s σ θ__σ
+    end. 
+    (*  *)
+    induction τ.
+    + (* CASE τ = 0 *)
+      intros;
+      lazymatch goal with
+      | [ Hexec: SitpnExecute _ _ _ _, Hsim: simloop _ _ _ _ _ _ _ |- _ ] =>
+        inversion_clear Hexec; inversion_clear Hsim; eauto
+      end.
+    + (* CASE τ > 0 *)
+      intros;
+      lazymatch goal with
+      | [ Hexec: SitpnExecute _ _ _ _, Hsim: simloop _ _ _ _ _ _ _ |- _ ] =>
+        inversion_clear Hexec; inversion_clear Hsim
+      end.
+      match goal with
+      | [ H1: simcycle _ _ _ _ _ _ _ _ |- _ ] =>
+        inversion_clear H1
+      end.
+      constructor. eapply rising_edge; eauto with hilecop.
+      constructor. eapply falling_edge; eauto with hilecop.
+      (* Apply the induction hypothesis. *)
+      eapply IHτ; eauto.
+      eapply falling_edge_full; eauto.
+      eapply rising_edge_full; eauto.
 Qed.
