test/sitpn/Example1.v
@@ -168,6 +168,6 @@ Example sitpn1 :=
 (* Require Import Sitpn2HVhdlTypes. *)
 (* Require Import String. *)
 
-(* Compute (sitpn_to_hvhdl sitpn1 prio1_dec 0 0 2). *)
+(* Compute (sitpn2hvhdl sitpn1 prio1_dec 0 0 2). *)
 
 
